Add inf_array_model'.

theories/std/inf_array.v
@@ -4,12 +4,12 @@ From Coq.Logic Require Import
 From caml5 Require Import
   prelude.
 From caml5.lang Require Import
-  notations.
+  notations
+  proofmode.
 From caml5.std Require Export
   base.
 
 Implicit Types t v : val.
-Implicit Types i : Z.
 
 Record inf_array `{!heapGS Σ} := {
   inf_array_make : val ;
@@ -46,13 +46,123 @@ Section inf_array.
   Context `{!heapGS Σ} (inf_array : inf_array Σ).
 
   #[global] Instance inf_array_model_ne t n :
-    Proper ((pointwise_relation nat (=)) ==> (≡{n}≡)) (inf_array.(inf_array_model) t).
+    Proper (pointwise_relation nat (=) ==> (≡{n}≡)) (inf_array.(inf_array_model) t).
   Proof.
     intros vs1 vs2 ->%functional_extensionality. done.
   Qed.
   #[global] Instance inf_array_model_proper t :
-    Proper ((pointwise_relation nat (=)) ==> (≡)) (inf_array.(inf_array_model) t).
+    Proper (pointwise_relation nat (=) ==> (≡)) (inf_array.(inf_array_model) t).
   Proof.
     intros vs1 vs2 Hvs. rewrite equiv_dist. solve_proper.
   Qed.
+
+  Definition inf_array_model' t vsₗ vsᵣ :=
+    inf_array.(inf_array_model) t (
+      λ i,
+        if decide (i < length vsₗ) then vsₗ !!! i else vsᵣ (i - length vsₗ)
+    ).
+
+  #[global] Instance inf_array_model'_ne t n :
+    Proper ((=) ==> pointwise_relation nat (=) ==> (≡{n}≡)) (inf_array_model' t).
+  Proof.
+    solve_proper.
+  Qed.
+  #[global] Instance inf_array_model'_proper t :
+    Proper ((=) ==> pointwise_relation nat (=) ==> (≡)) (inf_array_model' t).
+  Proof.
+    solve_proper.
+  Qed.
+
+  Lemma inf_array_get_spec' i t :
+    (0 ≤ i)%Z →
+    <<<
+      True |
+      ∀∀ vsₗ vsᵣ, inf_array_model' t vsₗ vsᵣ
+    >>>
+      inf_array.(inf_array_get) t #i
+    <<<
+      inf_array_model' t vsₗ vsᵣ |
+      RET
+        let i := Z.to_nat i in
+        if decide (i < length vsₗ) then vsₗ !!! i else vsᵣ (i - length vsₗ);
+      True
+    >>>.
+  Proof.
+    iIntros "% !> %Φ _ HΦ".
+    awp_apply (inf_array_get_spec with "[//]"); first done.
+    iApply (aacc_aupd with "HΦ"); first done.
+    iIntros "%vsₗ %vsᵣ Hmodel". iAaccIntro with "Hmodel"; first auto with iFrame.
+    iIntros "$ !>". iRight. iIntros "HΦ !> _". iApply ("HΦ" with "[//]").
+  Qed.
+
+  Lemma inf_array_set_spec' i v t :
+    (0 ≤ i)%Z →
+    <<<
+      True |
+      ∀∀ vsₗ vsᵣ, inf_array_model' t vsₗ vsᵣ
+    >>>
+      inf_array.(inf_array_set) t #i v
+    <<<
+      let i := Z.to_nat i in
+      if decide (i < length vsₗ)
+      then inf_array_model' t (<[i := v]> vsₗ) vsᵣ
+      else inf_array_model' t vsₗ (<[i - length vsₗ := v]> vsᵣ) |
+      RET #(); True
+    >>>.
+  Proof.
+    iIntros "% !> %Φ _ HΦ".
+    awp_apply (inf_array_set_spec with "[//]"); first done.
+    iApply (aacc_aupd with "HΦ"); first done.
+    iIntros "%vsₗ %vsᵣ Hmodel". iAaccIntro with "Hmodel"; first auto with iFrame.
+    iIntros "Hmodel !>". iRight. iSplitL "Hmodel".
+    - generalize (Z.to_nat i). clear. intros i. destruct (decide (i < length vsₗ)).
+      all: iApply (inf_array_model_proper with "Hmodel"); intros j.
+      + rewrite insert_length. destruct (decide (j < length vsₗ)).
+        * destruct (decide (j = i)) as [-> |].
+          -- rewrite list_lookup_total_insert // fn_lookup_insert //.
+          -- rewrite list_lookup_total_insert_ne // fn_lookup_insert_ne // decide_True //.
+        * rewrite fn_lookup_insert_ne; last lia.
+          rewrite decide_False //.
+      + destruct (decide (j < length vsₗ)).
+        * rewrite fn_lookup_insert_ne; last lia.
+          rewrite decide_True //.
+        * destruct (decide (j = i)) as [-> |].
+          -- rewrite !fn_lookup_insert //.
+          -- rewrite !fn_lookup_insert_ne; try lia.
+             rewrite decide_False //.
+    - iIntros "HΦ !> _". iApply ("HΦ" with "[//]").
+  Qed.
+
+  Lemma inf_array_model'_shift t vsₗ v vsᵣ :
+    inf_array_model' t (vsₗ ++ [v]) vsᵣ ⊣⊢
+    inf_array_model' t vsₗ (λ i, match i with 0 => v | S i => vsᵣ i end).
+  Proof.
+    rewrite /inf_array_model' inf_array_model_proper; first done.
+    intros j. rewrite app_length /=.
+    destruct (Nat.lt_total j (length vsₗ)) as [| [-> |]].
+    - rewrite !decide_True; try lia.
+      rewrite lookup_total_app_l //.
+    - rewrite decide_True; last lia.
+      rewrite decide_False; last lia.
+      rewrite lookup_total_app_r //.
+      rewrite Nat.sub_diag //.
+    - rewrite !decide_False; try lia.
+      case_match; [lia | f_equal; lia].
+  Qed.
+  Lemma inf_array_model'_shift_r t vsₗ v vsᵣ :
+    inf_array_model' t (vsₗ ++ [v]) vsᵣ -∗
+    inf_array_model' t vsₗ (λ i, match i with 0 => v | S i => vsᵣ i end).
+  Proof.
+    rewrite inf_array_model'_shift //.
+  Qed.
+  Lemma inf_array_model'_shift_l t vsₗ v vsᵣ :
+    inf_array_model' t vsₗ (λ i, match i with 0 => v | S i => vsᵣ i end) -∗
+    inf_array_model' t (vsₗ ++ [v]) vsᵣ.
+  Proof.
+    rewrite inf_array_model'_shift //.
+  Qed.
 End inf_array.
+
+Notation "inf_array .(inf_array_model')" := (inf_array_model' inf_array)
+( at level 5
+).
